examples/formal-languages/regular/regexp_compilerScript.sml
@@ -3,7 +3,7 @@ open optionTheory pairTheory relationTheory arithmeticTheory
      pred_setTheory bagTheory containerTheory
      listTheory rich_listTheory stringTheory sortingTheory mergesortTheory
      comparisonTheory balanced_mapTheory eq_cmp_bmapTheory osetTheory
-     finite_mapTheory vec_mapTheory charset64Theory regexpTheory
+     finite_mapTheory vec_mapTheory charsetTheory regexpTheory
 ;
 
 val _ = numLib.prefer_num();
@@ -666,10 +666,10 @@ CONJ_TAC
  >- rw_tac list_ss [SimpLHS, Once exec_dfa_def])
 
 (*
-val exec_dfa_def =
-  Define
+val exec_dfa_def = 
+  Define 
    `(exec_dfa finals table n [] = EL n finals) /\
-    (exec_dfa finals table n (c::t) =
+    (exec_dfa finals table n (c::t) = 
         case EL (ORD c) (EL n table) of
          | NONE => F
          | SOME k => exec_dfa finals table k t)`;
@@ -692,12 +692,12 @@ val regexp_matcher_def =
       exec_dfa acceptsV deltaV start_state`;
 
 (*
-val regexp_matcher_def =
- Define
-  `regexp_matcher r =
+val regexp_matcher_def = 
+ Define 
+  `regexp_matcher r = 
     let (state_numbering,delta,accepts) = compile_regexp r in
     let start_state_opt = balanced_map$lookup regexp_compare (normalize r) state_numbering
-    in
+    in 
       exec_dfa accepts delta (THE start_state_opt)`;
 *)
 
@@ -2138,3 +2138,4 @@ val Brzozowski_partial_eval_256 = save_thm
 (* val _ = EmitTeX.tex_theory"-"; *)
 
 val _ = export_theory();
+
